code/salsa-family/Salsa20.fst
@@ -1,19 +1,11 @@
 module Salsa20
 
-open FStar.Mul
-open FStar.HyperStack
-open FStar.ST
 open FStar.Buffer
-open Hacl.Cast
-open Hacl.UInt32
 open Hacl.Spec.Endianness
 open Hacl.Endianness
-open Spec.Salsa20
-open C.Loops
 
 open Hacl.Impl.Salsa20
-
-module Spec = Spec.Salsa20
+open Hacl.Impl.HSalsa20
 
 module U32 = FStar.UInt32
 module H8  = Hacl.UInt8
@@ -25,8 +17,7 @@ let uint8_p = buffer H8.t
 
 type state = b:Buffer.buffer h32{length b = 16}
 
-let value_at m (h:HyperStack.mem{live h m}) = reveal_sbytes (as_seq h m)
-
+let op_String_Access h (b:uint8_p{live h b}) = reveal_sbytes (as_seq h b)
 
 val salsa20:
   output:uint8_p ->
@@ -39,10 +30,17 @@ val salsa20:
     (requires (fun h -> live h output /\ live h plain /\ live h key /\ live h nonce))
     (ensures (fun h0 _ h1 -> live h1 output /\ live h0 plain /\ live h0 key /\ live h0 nonce
       /\ modifies_1 output h0 h1
-      /\ (let o = output `value_at` h1 in
-         let plain = plain `value_at` h0 in
-         let k = key `value_at` h0 in
-         let n = nonce `value_at` h0 in
-         let ctr = UInt64.v ctr in
-         o == Spec.Salsa20.salsa20_encrypt_bytes k n ctr plain)))
+      /\ (h1.[output] == Spec.Salsa20.salsa20_encrypt_bytes h0.[key] h0.[nonce] (UInt64.v ctr) h0.[plain])))
 let salsa20 output plain len k n ctr = salsa20 output plain len k n ctr
+
+val hsalsa20:
+  output:uint8_p{length output = 32} ->
+  key:uint8_p{length key = 32} ->
+  nonce:uint8_p{length nonce = 16} ->
+  Stack unit
+    (requires (fun h -> live h output /\ live h nonce /\ live h key))
+    (ensures  (fun h0 _ h1 -> live h0 output /\ live h0 nonce /\ live h0 key /\
+      modifies_1 output h0 h1 /\ live h1 output
+      /\ (h1.[output] == Spec.HSalsa20.hsalsa20 h0.[key] h0.[nonce])))
+let hsalsa20 output key nonce =
+  crypto_core_hsalsa20 output nonce key
