code/api/Hacl.SecretBox.fst
@@ -64,7 +64,7 @@ let crypto_secretbox_detached c mac m mlen n k =
   let mlen0_32 = Int.Cast.uint64_to_uint32 mlen0 in
   Math.Lemmas.modulo_lemma (U32.v mlen0_32) (pow2 32);
   blit m 0ul block0 zerobytes mlen0_32;
-  HSalsa20.hsalsa20 subkey k (sub n 0ul 16ul);
+  Salsa20.hsalsa20 subkey k (sub n 0ul 16ul);
   Salsa20.salsa20 block0 block0 (U32.(mlen0_32 +^ zerobytes)) subkey (sub n 16ul 8ul) 0uL;
   let h1 = ST.get() in
   cut (modifies_1 hsalsa_state h0' h1);
@@ -102,7 +102,7 @@ let crypto_secretbox_open_detached m c mac clen n k =
   let block0 = sub hsalsa_state 32ul 64ul in
   let tmp_mac = sub hsalsa_state 96ul 16ul in
   let h0' = ST.get() in
-  HSalsa20.hsalsa20 subkey k (sub n 0ul 16ul);
+  Salsa20.hsalsa20 subkey k (sub n 0ul 16ul);
   Salsa20.salsa20 block0 block0 32ul subkey (sub n 16ul 8ul) 0uL;
   let h1 = ST.get() in
   cut(modifies_0 h0 h1);
